finish source corrctness for pb checker

examples/pseudo_bool/array/npbc_fullProgScript.sml
@@ -9,13 +9,65 @@ val _ = translation_extends"npbc_parseProg";
 
 val xlet_autop = xlet_auto >- (TRY( xcon) >> xsimpl)
 
-Definition usage_string_def:
-  usage_string = strlit "Usage: cake_pb <OPB format formula file> <Proof file>\n"
-End
+(* TODO: move *)
+Theorem parse_constraint_LHS_goodString_aux:
+  ∀ls acc.
+  set (MAP (lit_var ∘ SND) acc) ⊆ goodString ⇒
+  set (MAP (lit_var ∘ SND) (SND (parse_constraint_LHS ls acc))) ⊆ goodString
+Proof
+  ho_match_mp_tac parse_constraint_LHS_ind>>
+  rw[parse_constraint_LHS_def]>>
+  fs[MAP_REVERSE]>>
+  every_case_tac>>fs[MAP_REVERSE]>>
+  pop_assum match_mp_tac>>
+  fs[parse_lit_def]>>
+  every_case_tac>>fs[]>>rw[]>>
+  metis_tac[SPECIFICATION]
+QED
 
-val r = translate usage_string_def;
+Theorem parse_constraint_LHS_goodString:
+  set (MAP (lit_var ∘ SND) (SND (parse_constraint_LHS ls []))) ⊆ goodString
+Proof
+  match_mp_tac parse_constraint_LHS_goodString_aux>>
+  fs[]
+QED
 
-(* additional translation for .pbf parsing *)
+Theorem parse_constraint_goodString:
+  parse_constraint h = SOME x ⇒
+  pbc_vars x ⊆ goodString
+Proof
+  rw[parse_constraint_def]>>
+  every_case_tac>>fs[]>>rw[]>>
+  fs[pbcTheory.pbc_vars_def]>>
+  metis_tac[parse_constraint_LHS_goodString,SND,parse_constraint_LHS_goodString]
+QED
+
+Theorem parse_constraints_goodString:
+  ∀ls acc pbf.
+  pbf_vars (set acc) ⊆ goodString ∧
+  parse_constraints ls acc = SOME pbf ⇒
+  pbf_vars (set pbf) ⊆ goodString
+Proof
+  Induct>>rw[parse_constraints_def]>>
+  simp[]>>
+  every_case_tac>>fs[]>>
+  first_x_assum (drule_at Any)>>
+  disch_then match_mp_tac>>
+  fs[pbcTheory.pbf_vars_def]>>
+  metis_tac[parse_constraint_goodString]
+QED
+
+Theorem parse_pbf_goodString:
+  parse_pbf ls = SOME pbf ⇒
+  pbf_vars (set pbf) ⊆ goodString
+Proof
+  fs[parse_pbf_def,parse_pbf_toks_def]>>
+  rw[]>>
+  (drule_at Any) parse_constraints_goodString>>
+  simp[pbcTheory.pbf_vars_def]
+QED
+
+(* Translation for parsing an OPB file *)
 val r = translate tokenize_def;
 val r = translate nocomment_line_def;
 
@@ -32,13 +84,6 @@ val strip_terminator_side = Q.prove(
   `∀x. strip_terminator_side x <=> T`,
   rw[strip_terminator_side_def])
   |> update_precondition;
-
-val r = translate flip_coeffs_def;
-val r = translate pbc_ge_def;
-val r = translate normalise_def;
-
-val r = translate convert_pbf_def;
-val r = translate full_normalise_def;
 
 val r = translate parse_op_def;
 val r = translate parse_constraint_def;
@@ -89,7 +134,7 @@ Theorem parse_pbf_full_spec:
     (POSTv v.
     & (∃err. (SUM_TYPE STRING_TYPE (LIST_TYPE (PAIR_TYPE PBC_PBOP_TYPE (PAIR_TYPE (LIST_TYPE (PAIR_TYPE INT (PBC_LIT_TYPE STRING_TYPE))) INT)))
     (if inFS_fname fs f then
-    (case parse_pbf_toks (MAP toks (all_lines fs f)) of
+    (case parse_pbf (all_lines fs f) of
       NONE => INL err
     | SOME x => INR x)
     else INL err) v)) * STDIO fs)
@@ -114,7 +159,7 @@ Proof
     xlet_autop>>
     `toks = (MAP tokenize ∘ tokens blanks)` by
       metis_tac[toks_def,ETA_AX,o_DEF]>>
-    rw[]>> TOP_CASE_TAC>>
+    rw[parse_pbf_def]>> TOP_CASE_TAC>>
     fs[OPTION_TYPE_def]
     >- (
       xmatch >>
@@ -129,62 +174,152 @@ Proof
   simp[SUM_TYPE_def]>>metis_tac[]
 QED
 
+val r = translate parse_header_line_fast_def;
+
+Definition check_f_line_def:
+  (check_f_line [] = F) ∧
+  (check_f_line ((s: mlstring + int)::ss) ⇔ s = INL (strlit "f"))
+End
+
+val r = translate check_f_line_def;
+
+Definition check_header_full_def:
+  check_header_full s s' =
+  case s of NONE => SOME 0
+  | SOME s =>
+  case s' of NONE => SOME 1
+  | SOME s' =>
+  if parse_header_line_fast s then
+    if check_f_line s' then NONE
+    else SOME (1:num)
+  else SOME 0
+End
+
+val r = translate check_header_full_def;
+
+val check_header = process_topdecs`
+  fun check_header fd =
+      check_header_full
+        (TextIO.b_inputLineTokens fd blanks tokenize_fast)
+        (TextIO.b_inputLineTokens fd blanks tokenize_fast)` |> append_prog;
+
+val b_inputLineTokens_specialize =
+  b_inputLineTokens_spec_lines
+  |> Q.GEN `f` |> Q.SPEC`blanks`
+  |> Q.GEN `fv` |> Q.SPEC`blanks_v`
+  |> Q.GEN `g` |> Q.ISPEC`tokenize_fast`
+  |> Q.GEN `gv` |> Q.ISPEC`tokenize_fast_v`
+  |> Q.GEN `a` |> Q.ISPEC`SUM_TYPE STRING_TYPE INT`
+  |> SIMP_RULE std_ss [blanks_v_thm,tokenize_fast_v_thm,blanks_def] ;
+
+Theorem check_header_spec:
+  !ss fd fdv lines fs.
+  app (p : 'ffi ffi_proj)
+    ^(fetch_v "check_header" (get_ml_prog_state()))
+    [fdv]
+    (STDIO fs * INSTREAM_LINES fd fdv lines fs)
+    (POSTv v.
+       SEP_EXISTS k lines' res.
+       STDIO (forwardFD fs fd k) *
+       INSTREAM_LINES fd fdv lines' (forwardFD fs fd k) *
+       &(OPTION_TYPE NUM res v))
+Proof
+  xcf "check_header" (get_ml_prog_state ())>>
+  rpt xlet_autop>>
+  xlet ‘(POSTv v.
+      SEP_EXISTS k.
+          STDIO (forwardFD fs fd k) *
+          INSTREAM_LINES fd fdv (TL lines) (forwardFD fs fd k) *
+          &OPTION_TYPE (LIST_TYPE (SUM_TYPE STRING_TYPE INT))
+            (OPTION_MAP (MAP tokenize_fast ∘ tokens blanks) (oHD lines)) v)’
+  >- (
+    xapp_spec b_inputLineTokens_specialize
+    \\ qexists_tac ‘emp’
+    \\ xsimpl)>>
+  xlet ‘(POSTv v.
+      SEP_EXISTS k.
+          STDIO (forwardFD fs fd k) *
+          INSTREAM_LINES fd fdv (TL (TL lines)) (forwardFD fs fd k) *
+          &OPTION_TYPE (LIST_TYPE (SUM_TYPE STRING_TYPE INT))
+            (OPTION_MAP (MAP tokenize_fast ∘ tokens blanks) (oHD (TL lines))) v)’
+  >- (
+    xapp_spec b_inputLineTokens_specialize
+    \\ qexists_tac ‘emp’
+    \\ xsimpl
+    \\ metis_tac[forwardFD_o,STDIO_INSTREAM_LINES_refl,STDIO_INSTREAM_LINES_refl_gc]
+    )>>
+  xapp>>
+  xsimpl>>
+  metis_tac[forwardFD_o,STDIO_INSTREAM_LINES_refl,STDIO_INSTREAM_LINES_refl_gc]
+QED
+
+Definition success_string_def:
+  success_string = strlit "Verified\n"
+End
+
+val r = translate success_string_def;
+
 Definition result_string_def:
-  result_string b =
-   if b
-   then INR (strlit "Verified\n")
-   else INL (strlit "Proof checking succeeded but did not derive contradiction\n")
+  result_string ob =
+   case ob of
+    INR b =>
+      if b then INR success_string
+      else INL (strlit "Proof checking succeeded but did not derive contradiction\n")
+  | INL v => INL v
 End
 
 val r = translate result_string_def;
 
-val check_unsat' = process_topdecs `
-  fun check_unsat' fml inds id fname =
+val check_unsat_top = process_topdecs `
+  fun check_unsat_top fml fname =
   let
     val fd = TextIO.b_openIn fname
-    val u = (check_header fd;
-      case check_unsat'' fd 1 fml inds id of
-        (fml', (b, (id',inds'))) => result_string b
-      ) handle Fail s => Inl s
-    val close = TextIO.b_closeIn fd;
   in
-    u
+    case check_header fd of
+      Some n =>
+      (TextIO.b_closeIn fd;
+      Inl (format_failure n "Unable to parse header"))
+    | None =>
+      let val res =
+        result_string (check_unsat fd 2 fml)
+        val close = TextIO.b_closeIn fd;
+      in
+        res
+      end
   end
   handle TextIO.BadFileName => Inl (notfound_string fname)` |> append_prog;
 
-(*
-Definition parse_pbp_def:
-  parse_pbp strs =
-  case MAP toks_fast strs of
-    s::ss =>
-    if parse_header_line_fast s then
-      parse_tops ss
-    else NONE
-  | [] => NONE
-End *)
+Theorem STDIO_INSTREAM_LINES_refl_more_gc:
+  STDIO A *
+  INSTREAM_LINES B C D E * rest ==>>
+  STDIO A *
+  INSTREAM_LINES B C D E * GC
+Proof
+  xsimpl
+QED
 
-(* Dummy spec *)
-Theorem check_unsat'_spec:
-  SPTREE_SPT_TYPE PB_CONSTRAINT_NPBC_TYPE fml fmlv ∧ NUM id idv ∧
+Theorem check_unsat_top_spec:
+  LIST_TYPE
+    (PAIR_TYPE PBC_PBOP_TYPE
+       (PAIR_TYPE (LIST_TYPE (PAIR_TYPE INT (PBC_LIT_TYPE STRING_TYPE)))
+          INT)) fml fmlv ∧
   FILENAME f fv ∧
-  hasFreeFD fs
+  hasFreeFD fs ∧
+  pbf_vars (set fml) ⊆ goodString
   ⇒
-  app (p:'ffi ffi_proj) ^(fetch_v"check_unsat'"(get_ml_prog_state()))
-  [fmlv; idv; fv]
+  app (p:'ffi ffi_proj) ^(fetch_v"check_unsat_top"(get_ml_prog_state()))
+  [fmlv; fv]
   (STDIO fs)
   (POSTv v.
-    STDIO fs *
-    SEP_EXISTS err.
-      &(SUM_TYPE STRING_TYPE (OPTION_TYPE (LIST_TYPE INT)))
-      (if inFS_fname fs f then
-        ARB
-      else
-        INL err
-      ) v)
+     STDIO fs *
+     SEP_EXISTS res.
+     &(
+      SUM_TYPE STRING_TYPE STRING_TYPE res v ∧
+      (∀s. res = INR s ⇒
+        (s = success_string ∧
+        unsatisfiable (set fml)))))
 Proof
-  cheat
-  (*
-  xcf"check_unsat'"(get_ml_prog_state()) >>
+  xcf"check_unsat_top"(get_ml_prog_state()) >>
   reverse (Cases_on `STD_streams fs`)
   >- (fs [TextIOProofTheory.STDIO_def] \\ xpull) >>
   reverse (Cases_on`consistentFS fs`)
@@ -202,120 +337,117 @@ Proof
       xcases>>rw[]>>
       xlet_auto>>xsimpl>>
       xcon>>xsimpl>>
-      simp[SUM_TYPE_def]>>metis_tac[])>>
+      qexists_tac`INL (notfound_string f)`>>
+      simp[SUM_TYPE_def])>>
   qmatch_goalsub_abbrev_tac`$POSTv Qval`>>
   xhandle`$POSTv Qval` \\ xsimpl >>
   qunabbrev_tac`Qval`>>
   xlet_auto_spec (SOME b_openIn_spec_lines) \\ xsimpl >>
-  xlet`POSTv resv.
-        SEP_EXISTS k rest.
-         STDIO (forwardFD fs (nextFD fs) k) *
-         INSTREAM_LINES (nextFD fs) is rest (forwardFD fs (nextFD fs) k) *
-         &(
-           ARB
-           (* case
-             parse_and_run_file_list (all_lines fs f) fmlls ls (REPLICATE n w8z) earliest
-           of
-             NONE => resv = Conv (SOME (TypeStamp "Inl" 23)) [v0] ∧ ∃s. STRING_TYPE s v0
-           | SOME(fmlls',inds') =>
-             resv = Conv (SOME (TypeStamp "Inr" 23)) [Conv NONE [v1; v2]] ∧
-             v1 = fmlv' ∧
-             LIST_REL (OPTION_TYPE (LIST_TYPE INT)) fmlls' fmllsv' ∧ LIST_TYPE NUM inds' v2 *)
-         )`
-  >-
-    cheat
-  >>
-  cheat *)
+  qmatch_goalsub_abbrev_tac`INSTREAM_LINES fd fdv lines fss`>>
+  xlet`POSTv v.
+    SEP_EXISTS k lines' res.
+    STDIO (forwardFD fss fd k) *
+    INSTREAM_LINES fd fdv lines' (forwardFD fss fd k) *
+    &OPTION_TYPE NUM res v`
+  >- (
+    xapp>>
+    qexists_tac`emp`>>
+    xsimpl>>
+    metis_tac[STDIO_INSTREAM_LINES_refl,STDIO_INSTREAM_LINES_refl_gc,STAR_COMM])>>
+  qmatch_goalsub_abbrev_tac`INSTREAM_LINES fd fdv _ fsss`>>
+  reverse (Cases_on`res`)>>fs[OPTION_TYPE_def]>>xmatch
+  >- (
+    xlet `POSTv v. STDIO fs`
+    >- (
+      xapp_spec b_closeIn_spec_lines >>
+      xsimpl>>
+      qexists_tac `emp`>>
+      qexists_tac `lines'` >>
+      qexists_tac `fsss`>>
+      qexists_tac `fd` >>
+      conj_tac THEN1
+        (unabbrev_all_tac
+        \\ imp_res_tac fsFFIPropsTheory.nextFD_ltX \\ fs []
+        \\ imp_res_tac fsFFIPropsTheory.STD_streams_nextFD \\ fs []) >>
+      xsimpl>>
+      `validFileFD fd fsss.infds` by
+        (unabbrev_all_tac>> simp[validFileFD_forwardFD]
+         \\ imp_res_tac fsFFIPropsTheory.nextFD_ltX \\ fs []
+         \\ match_mp_tac validFileFD_nextFD \\ fs []) >>
+      xsimpl >> rw [] >>
+      unabbrev_all_tac>>xsimpl>>
+      simp[forwardFD_ADELKEY_same]>>
+      DEP_REWRITE_TAC [fsFFIPropsTheory.openFileFS_ADELKEY_nextFD]>>
+      xsimpl>>
+      imp_res_tac (DECIDE ``n<m:num ==> n <= m``) >>
+      imp_res_tac fsFFIPropsTheory.nextFD_leX \\ fs [])>>
+    xlet_autop>>
+    xcon>>
+    xsimpl>>
+    metis_tac[SUM_TYPE_def,sum_distinct])>>
+  xlet`POSTv v. SEP_EXISTS k lines' lno' fmlv' fmllsv' res.
+          STDIO (forwardFD fsss fd k) *
+          INSTREAM_LINES fd fdv lines' (forwardFD fsss fd k) *
+          &(SUM_TYPE STRING_TYPE BOOL res v ∧
+           (res = INR T ⇒ unsatisfiable (set fml)))`
+  >- (
+    xapp>>xsimpl>>
+    qexists_tac`emp`>>xsimpl>>
+    metis_tac[STDIO_INSTREAM_LINES_refl_more_gc,STDIO_INSTREAM_LINES_refl])>>
+  xlet_autop>>
+  xlet `POSTv v. STDIO fs`
+  >- (
+    xapp_spec b_closeIn_spec_lines >>
+    xsimpl>>
+    qexists_tac `emp`>>
+    qexists_tac `lines'` >>
+    qexists_tac `forwardFD fsss fd k'`>>
+    qexists_tac `fd` >>
+    conj_tac THEN1
+      (unabbrev_all_tac
+      \\ imp_res_tac fsFFIPropsTheory.nextFD_ltX \\ fs []
+      \\ imp_res_tac fsFFIPropsTheory.STD_streams_nextFD \\ fs []) >>
+    xsimpl>>
+    `validFileFD fd (forwardFD fsss fd k').infds` by
+      (unabbrev_all_tac>> simp[validFileFD_forwardFD]
+       \\ imp_res_tac fsFFIPropsTheory.nextFD_ltX \\ fs []
+       \\ match_mp_tac validFileFD_nextFD \\ fs []) >>
+    xsimpl >> rw [] >>
+    unabbrev_all_tac>>xsimpl>>
+    simp[forwardFD_ADELKEY_same]>>
+    DEP_REWRITE_TAC [fsFFIPropsTheory.openFileFS_ADELKEY_nextFD]>>
+    xsimpl>>
+    imp_res_tac (DECIDE ``n<m:num ==> n <= m``) >>
+    imp_res_tac fsFFIPropsTheory.nextFD_leX \\ fs [])>>
+  xvar>>xsimpl>>
+  asm_exists_tac>>fs[]>>
+  Cases_on`res`>>gs[result_string_def]
 QED
-
-val _ = translate miscTheory.enumerate_def;
-
-val fill_arr = process_topdecs`
-  fun fill_arr arr ls =
-    case ls of [] => arr
-    | (x::xs) =>
-    case x of (i,v) =>
-      fill_arr (Array.updateResize arr None i (Some v)) xs` |> append_prog
-
-(*
-Theorem fill_arr_spec:
-  ∀ls lsv arrv arrls arrlsv.
-  LIST_TYPE (PAIR_TYPE NUM (LIST_TYPE INT)) ls lsv ∧
-  LIST_REL (OPTION_TYPE (LIST_TYPE INT)) arrls arrlsv
-  ⇒
-  app (p:'ffi ffi_proj) ^(fetch_v"fill_arr"(get_ml_prog_state()))
-  [arrv; lsv]
-  (ARRAY arrv arrlsv)
-  (POSTv resv.
-  SEP_EXISTS arrlsv'. ARRAY resv arrlsv' *
-    & LIST_REL (OPTION_TYPE (LIST_TYPE INT)) (FOLDL (λacc (i,v).  update_resize acc NONE (SOME v) i) arrls ls) arrlsv')
-Proof
-  Induct>>rw[]>>
-  xcf "fill_arr" (get_ml_prog_state ())>>
-  fs[LIST_TYPE_def]>>
-  xmatch
-  >- (xvar>>xsimpl)>>
-  Cases_on`h`>>fs[PAIR_TYPE_def]>>
-  xmatch>>
-  rpt xlet_autop >>
-  xlet_auto >>
-  xapp>>
-  fs[]>>
-  match_mp_tac LIST_REL_update_resize>>fs[]>>
-  simp[OPTION_TYPE_def]
-QED
-val _ = translate build_fml_def;
-
-Definition build_def:
-  build pbf = build_fml 1 (full_normalise pbf) LN
-End
-
-val r = translate build_def;
-
-val check_pbp = process_topdecs`
-  fun check_pbp pbf fname =
-    case build pbf of (fml,id) =>
-    check_unsat' fml id fname` |> append_prog;
-*)
 
 val check_unsat_2 = (append_prog o process_topdecs) `
   fun check_unsat_2 f1 f2 =
   case parse_pbf_full f1 of
     Inl err => TextIO.output TextIO.stdErr err
   | Inr fml =>
-  let val ls = enumerate 1 (full_normalise fml)
-      val id = List.length ls + 1
-      val arr = Array.array (2*id) None
-      val arr = fill_arr arr ls
-      val inds = []
-  in
-    case check_unsat' arr inds id f2 of
+    (case check_unsat_top fml f2 of
       Inl err => TextIO.output TextIO.stdErr err
-    | Inr s => TextIO.print s
-  end`
+    | Inr s => TextIO.print s)`
 
-val check_unsat_2_sem_def = Define`
-  check_unsat_2_sem fs f1 f2 err =
-  if inFS_fname fs f1 then
-  (case parse_pbf_toks (MAP toks (all_lines fs f1)) of
-    NONE => add_stderr fs err
-  | SOME pbf =>
-    if inFS_fname fs f2 then
-      ARB (* case parse_pbp_toks (MAP toks (all_lines fs f2)) of
-        SOME pbp =>
-        ARB
-        (* case check_pbp pbf pbp of
-          INL _ => add_stderr fs err
-        | INR succ => add_stdout fs succ *)
-      | NONE => add_stderr fs err *)
-    else add_stderr fs err)
-  else add_stderr fs err`
+Theorem success_string_not_nil:
+  strlit "" ≠ success_string
+Proof
+  EVAL_TAC
+QED
 
-val err_tac = xapp_spec output_stderr_spec \\ xsimpl>>
-    asm_exists_tac>>xsimpl>>
-    qexists_tac`emp`>>xsimpl>>
-    qexists_tac`fs`>>xsimpl>>
-    rw[]>>qexists_tac`err`>>xsimpl;
+Definition check_unsat_2_sem_def:
+  check_unsat_2_sem fs f1 out ⇔
+  if out = success_string then
+    inFS_fname fs f1 ∧
+    ∃fml.
+    parse_pbf (all_lines fs f1) = SOME fml ∧
+    unsatisfiable (set fml)
+  else out = strlit""
+End
 
 Theorem check_unsat_2_spec:
   STRING_TYPE f1 f1v ∧ validArg f1 ∧
@@ -326,130 +458,268 @@ Theorem check_unsat_2_spec:
     [f1v; f2v]
     (STDIO fs)
     (POSTv uv. &UNIT_TYPE () uv *
-    SEP_EXISTS err. STDIO (check_unsat_2_sem fs f1 f2 err))
+    SEP_EXISTS out err.
+      STDIO (add_stdout (add_stderr fs err) out) *
+      &(check_unsat_2_sem fs f1 out))
 Proof
-  cheat
-  (*
-  rw[]>>
+  rw[check_unsat_2_sem_def]>>
   xcf "check_unsat_2" (get_ml_prog_state ())>>
+  reverse (Cases_on `STD_streams fs`) >- (fs [TextIOProofTheory.STDIO_def] \\ xpull) >>
   xlet_autop>>
-  simp[check_unsat_2_sem_def]>>
-  reverse TOP_CASE_TAC>>fs[]
+  pop_assum mp_tac>>
+  reverse IF_CASES_TAC
   >- (
-    fs[SUM_TYPE_def]>>xmatch>>
-    err_tac)>>
-  TOP_CASE_TAC>> fs[SUM_TYPE_def]
-  >- (xmatch>> err_tac)>>
-  xmatch>>
-  xlet_autop>>
-  reverse TOP_CASE_TAC>>fs[]
-  >- (
-    fs[SUM_TYPE_def]>>xmatch>>
-    err_tac)>>
-  TOP_CASE_TAC>> fs[SUM_TYPE_def]
-  >- (xmatch>>err_tac)>>
-  xmatch>>
-  xlet_autop>>
-  TOP_CASE_TAC >> fs[SUM_TYPE_def]
-  >- (xmatch >>
+    simp[SUM_TYPE_def]>>rw[]>>
+    xmatch>>
     xapp_spec output_stderr_spec \\ xsimpl>>
     asm_exists_tac>>xsimpl>>
     qexists_tac`emp`>>xsimpl>>
     qexists_tac`fs`>>xsimpl>>
-    rw[]>>qexists_tac`x''`>>xsimpl)>>
+    rw[]>>
+    qexists_tac`err`>>xsimpl>>rw[]>>
+    fs[success_string_not_nil,STD_streams_add_stderr, STD_streams_stdout,add_stdo_nil]>>
+    xsimpl)>>
+  TOP_CASE_TAC
+  >- (
+    simp[SUM_TYPE_def]>>rw[]>>
+    xmatch>>
+    xapp_spec output_stderr_spec \\ xsimpl>>
+    asm_exists_tac>>xsimpl>>
+    qexists_tac`emp`>>xsimpl>>
+    qexists_tac`fs`>>xsimpl>>
+    rw[]>>
+    qexists_tac`err`>>xsimpl>>rw[]>>
+    fs[success_string_not_nil,STD_streams_add_stderr, STD_streams_stdout,add_stdo_nil]>>
+    xsimpl)>>
+  simp[SUM_TYPE_def]>>rw[]>>
   xmatch>>
-  xapp_spec print_spec >> xsimpl
-  \\ qexists_tac`emp`
-  \\ asm_exists_tac \\ xsimpl
-  \\ qexists_tac`fs`>>xsimpl*)
+  drule parse_pbf_goodString>>
+  strip_tac>>
+  xlet`POSTv v.
+     STDIO fs *
+     SEP_EXISTS res.
+     &(
+      SUM_TYPE STRING_TYPE STRING_TYPE res v ∧
+      (∀s. res = INR s ⇒
+        (s = success_string ∧
+        unsatisfiable (set x))))`
+  >- (
+    xapp>>xsimpl>>
+    fs[FILENAME_def,validArg_def]>>
+    metis_tac[])>>
+  Cases_on`res`>>fs[SUM_TYPE_def]>>xmatch
+  >- (
+    xapp_spec output_stderr_spec \\ xsimpl>>
+    asm_exists_tac>>xsimpl>>
+    qexists_tac`emp`>>xsimpl>>
+    qexists_tac`fs`>>xsimpl>>
+    rw[]>>
+    qexists_tac`strlit ""`>>
+    qexists_tac`x'`>>xsimpl>>rw[]>>
+    fs[success_string_not_nil,STD_streams_add_stderr, STD_streams_stdout,add_stdo_nil]>>
+    xsimpl)>>
+  xapp>>asm_exists_tac>>xsimpl>>
+  qexists_tac`emp`>>qexists_tac`fs`>>xsimpl>>
+  rw[]>>
+  qexists_tac`success_string`>>simp[]>>
+  qexists_tac`strlit ""`>>
+  simp[STD_streams_stderr,add_stdo_nil]>>
+  xsimpl
 QED
 
-val check_unsat = (append_prog o process_topdecs) `
-  fun check_unsat u =
-  case CommandLine.arguments () of
-    [f1,f2] => check_unsat_2 f1 f2
-  | _ => TextIO.output TextIO.stdErr usage_string`
+Definition print_pbf_def:
+  print_pbf f = MAP pbc_string f
+End
 
-val check_unsat_sem_def = Define`
-  check_unsat_sem cl fs err =
-  case TL cl of
-  | [f1;f2] => check_unsat_2_sem fs f1 f2 err
-  | _ => add_stderr fs err`
+val res = translate pb_parseTheory.lit_string_def;
+val res = translate pb_parseTheory.lhs_string_def;
+val res = translate pb_parseTheory.op_string_def;
+val res = translate pb_parseTheory.pbc_string_def;
+val res = translate print_pbf_def;
 
-Theorem check_unsat_spec:
+val check_unsat_1 = (append_prog o process_topdecs) `
+  fun check_unsat_1 f1 =
+    case parse_pbf_full f1 of
+    Inl err => TextIO.output TextIO.stdErr err
+  | Inr fml =>
+  TextIO.print_list (print_pbf fml)`
+
+Definition check_unsat_1_sem_def:
+  check_unsat_1_sem fs f1 out ⇔
+  if inFS_fname fs f1
+  then
+    case parse_pbf (all_lines fs f1) of
+      NONE => out = strlit ""
+    | SOME fml => out = concat (print_pbf fml)
+  else out = strlit ""
+End
+
+Theorem check_unsat_1_spec:
+  STRING_TYPE f1 f1v ∧ validArg f1 ∧
   hasFreeFD fs
   ⇒
-  app (p:'ffi ffi_proj) ^(fetch_v"check_unsat"(get_ml_prog_state()))
+  app (p:'ffi ffi_proj) ^(fetch_v"check_unsat_1"(get_ml_prog_state()))
+    [f1v]
+    (STDIO fs)
+    (POSTv uv. &UNIT_TYPE () uv *
+    SEP_EXISTS out err.
+      STDIO (add_stdout (add_stderr fs err) out) *
+      &(check_unsat_1_sem fs f1 out))
+Proof
+  rw[check_unsat_1_sem_def]>>
+  xcf "check_unsat_1" (get_ml_prog_state ())>>
+  reverse (Cases_on `STD_streams fs`) >- (fs [TextIOProofTheory.STDIO_def] \\ xpull) >>
+  xlet_autop>>
+  pop_assum mp_tac>>
+  reverse IF_CASES_TAC
+  >- (
+    simp[SUM_TYPE_def]>>rw[]>>
+    xmatch>>
+    xapp_spec output_stderr_spec \\ xsimpl>>
+    asm_exists_tac>>xsimpl>>
+    qexists_tac`emp`>>qexists_tac`fs`>>xsimpl>>
+    fs[success_string_not_nil,STD_streams_add_stderr, STD_streams_stdout,add_stdo_nil]>>
+    rw[]>>
+    qexists_tac`err`>>xsimpl)>>
+  TOP_CASE_TAC>>fs[SUM_TYPE_def]>>rw[]>>xmatch
+  >- (
+    xapp_spec output_stderr_spec \\ xsimpl>>
+    asm_exists_tac>>xsimpl>>
+    qexists_tac`emp`>>qexists_tac`fs`>>xsimpl>>
+    fs[success_string_not_nil,STD_streams_add_stderr, STD_streams_stdout,add_stdo_nil]>>
+    rw[]>>
+    qexists_tac`err`>>xsimpl)>>
+  xlet_autop>>
+  xapp_spec print_list_spec>>xsimpl>>
+  asm_exists_tac>>xsimpl>>
+  qexists_tac`emp`>>qexists_tac`fs`>>xsimpl>>
+  rw[]>>
+  qexists_tac`strlit ""`>>
+  simp[STD_streams_stderr,add_stdo_nil]>>
+  xsimpl
+QED
+
+Definition usage_string_def:
+  usage_string = strlit "Usage: cake_pb <OPB file> <optional: proof file>\n"
+End
+
+val r = translate usage_string_def;
+
+val main = (append_prog o process_topdecs) `
+  fun main u =
+  case CommandLine.arguments () of
+    [f1] => check_unsat_1 f1
+  | [f1,f2] => check_unsat_2 f1 f2
+  | _ => TextIO.output TextIO.stdErr usage_string`
+
+Definition main_sem_def:
+  main_sem fs cl out =
+  if LENGTH cl = 2 then
+    check_unsat_1_sem fs (EL 1 cl) out
+  else if LENGTH cl = 3 then
+    check_unsat_2_sem fs (EL 1 cl) out
+  else out = strlit ""
+End
+
+Theorem STDIO_refl:
+  STDIO A ==>>
+  STDIO A * GC
+Proof
+  xsimpl
+QED
+
+Theorem main_spec:
+  hasFreeFD fs
+  ⇒
+  app (p:'ffi ffi_proj) ^(fetch_v"main"(get_ml_prog_state()))
     [Conv NONE []]
     (COMMANDLINE cl * STDIO fs)
     (POSTv uv. &UNIT_TYPE () uv *
-    COMMANDLINE cl * SEP_EXISTS err. STDIO (check_unsat_sem cl fs err))
+    COMMANDLINE cl *
+    SEP_EXISTS out err.
+      STDIO (add_stdout (add_stderr fs err) out) *
+      &(main_sem fs cl out))
 Proof
-  xcf"check_unsat"(get_ml_prog_state())>>
+  rw[main_sem_def]>>
+  xcf"main"(get_ml_prog_state())>>
+  reverse (Cases_on `STD_streams fs`) >- (fs [TextIOProofTheory.STDIO_def] \\ xpull) >>
   reverse(Cases_on`wfcl cl`) >- (fs[COMMANDLINE_def] \\ xpull)>>
   rpt xlet_autop >>
   Cases_on `cl` >- fs[wfcl_def] >>
-  simp[check_unsat_sem_def]>>
-  every_case_tac>>fs[LIST_TYPE_def]>>xmatch>>
-  qmatch_asmsub_abbrev_tac`wfcl cl`
+  Cases_on`t`>>fs[LIST_TYPE_def]
   >- (
+    xmatch>>
     xapp_spec output_stderr_spec \\ xsimpl>>
+    rename1`COMMANDLINE cl`>>
     qexists_tac`COMMANDLINE cl`>>xsimpl>>
-    qexists_tac `usage_string` >> simp [theorem "usage_string_v_thm"] >>
+    qexists_tac `usage_string` >>
+    simp [theorem "usage_string_v_thm"] >>
     qexists_tac`fs`>>xsimpl>>
-    rw[]>>qexists_tac`usage_string`>>xsimpl)
+    rw[]>>
+    fs[success_string_not_nil,STD_streams_add_stderr, STD_streams_stdout,add_stdo_nil]>>
+    metis_tac[STDIO_refl])>>
+  Cases_on`t'`>>fs[LIST_TYPE_def]
   >- (
-    xapp_spec output_stderr_spec \\ xsimpl>>
-    qexists_tac`COMMANDLINE cl`>>xsimpl>>
-    qexists_tac `usage_string` >> simp [theorem "usage_string_v_thm"] >>
-    qexists_tac`fs`>>xsimpl>>
-    rw[]>>qexists_tac`usage_string`>>xsimpl)
+    xmatch>>
+    xapp>>fs[]>>
+    rw[]>>
+    fs[wfcl_def]>>
+    first_x_assum (irule_at Any)>>xsimpl>>
+    first_x_assum (irule_at Any)>>xsimpl>>
+    rw[]>>
+    metis_tac[STDIO_refl])>>
+  Cases_on`t`>>fs[LIST_TYPE_def]
   >- (
-    xapp>>xsimpl>>
-    qexists_tac`COMMANDLINE cl`>>xsimpl>>
-    fs[wfcl_def,Abbr`cl`]>>
-    qexists_tac`fs`>>xsimpl>>
-    qexists_tac`h''`>>
-    qexists_tac`h'`>>
-    xsimpl>>rw[]>>
-    qexists_tac`x`>>xsimpl)
-  >- (
-    xapp_spec output_stderr_spec \\ xsimpl>>
-    qexists_tac`COMMANDLINE cl`>>xsimpl>>
-    qexists_tac `usage_string` >> simp [theorem "usage_string_v_thm"] >>
-    qexists_tac`fs`>>xsimpl>>
-    rw[]>>qexists_tac`usage_string`>>xsimpl)
+    xmatch>>
+    xapp>>rw[]>>
+    first_x_assum (irule_at Any)>>xsimpl>>
+    first_x_assum (irule_at Any)>>xsimpl>>
+    first_x_assum (irule_at Any)>>xsimpl>>
+    fs[wfcl_def]>>
+    rw[]>>metis_tac[STDIO_refl])>>
+  xmatch>>
+  xapp_spec output_stderr_spec \\ xsimpl>>
+  rename1`COMMANDLINE cl`>>
+  qexists_tac`COMMANDLINE cl`>>xsimpl>>
+  qexists_tac `usage_string` >>
+  simp [theorem "usage_string_v_thm"] >>
+  qexists_tac`fs`>>xsimpl>>
+  rw[]>>
+  fs[success_string_not_nil,STD_streams_add_stderr, STD_streams_stdout,add_stdo_nil]>>
+  metis_tac[STDIO_refl]
 QED
 
-Theorem check_unsat_whole_prog_spec2:
+Theorem main_whole_prog_spec2:
    hasFreeFD fs ⇒
-   whole_prog_spec2 check_unsat_v cl fs NONE (λfs'. ∃err. fs' = check_unsat_sem cl fs err)
+   whole_prog_spec2 main_v cl fs NONE
+     (λfs'. ∃out err.
+        fs' = add_stdout (add_stderr fs err) out ∧
+        main_sem fs cl out)
 Proof
-  cheat
-  (* rw[basis_ffiTheory.whole_prog_spec2_def]
-  \\ match_mp_tac (MP_CANON (DISCH_ALL (MATCH_MP app_wgframe (UNDISCH check_unsat_spec))))
+  rw[basis_ffiTheory.whole_prog_spec2_def]
+  \\ match_mp_tac (MP_CANON (DISCH_ALL (MATCH_MP app_wgframe (UNDISCH main_spec))))
   \\ xsimpl
   \\ rw[PULL_EXISTS]
-  \\ qexists_tac`check_unsat_sem cl fs x`
-  \\ qexists_tac`x`
+  \\ qexists_tac`add_stdout (add_stderr fs x') x`
   \\ xsimpl
-  \\ rw[check_unsat_sem_def,check_unsat_2_sem_def]
-  \\ every_case_tac
-  \\ simp[GSYM add_stdo_with_numchars,with_same_numchars] *)
+  \\ qexists_tac`x`
+  \\ qexists_tac`x'`
+  \\ xsimpl
+  \\ simp[GSYM add_stdo_with_numchars,with_same_numchars]
 QED
 
 local
 
-val name = "check_unsat"
+val name = "main"
 val (sem_thm,prog_tm) =
-  whole_prog_thm (get_ml_prog_state()) name (UNDISCH check_unsat_whole_prog_spec2)
-val check_unsat_prog_def = Define`check_unsat_prog = ^prog_tm`;
+  whole_prog_thm (get_ml_prog_state()) name (UNDISCH main_whole_prog_spec2)
+val main_prog_def = Define`main_prog = ^prog_tm`;
 
 in
 
-Theorem check_unsat_semantics =
+Theorem main_semantics =
   sem_thm
-  |> REWRITE_RULE[GSYM check_unsat_prog_def]
+  |> REWRITE_RULE[GSYM main_prog_def]
   |> DISCH_ALL
   |> SIMP_RULE(srw_ss())[GSYM CONJ_ASSOC,AND_IMP_INTRO];
 
